


1. Beta - Binomial conjugation:

proof: For convenience, we take coin tossing as an example.

Assume that we toss a coin N times, with m times resulting in heads.

Previously, there have been a heads a times and tails b times.

Denote the probability of tossing heads by θ .

$$\text{Then } p(\theta | \text{event}) = \frac{P(\text{event} | \theta) \cdot P(\theta)}{P(\text{event})}$$

$$(*) = \frac{\cancel{\binom{N}{m}} \cdot \theta^m \cdot (1-\theta)^{N-m} \cdot \theta^{a-1} \cdot (1-\theta)^{b-1} \cdot \cancel{\frac{\Gamma(a+b)}{\Gamma(a) \cdot \Gamma(b)}}}{\int_0^1 \cancel{\binom{N}{m}} \cdot \theta^m \cdot (1-\theta)^{N-m} \cdot \theta^{a-1} \cdot (1-\theta)^{b-1} \cdot \cancel{\frac{\Gamma(a+b)}{\Gamma(a) \Gamma(b)}} d\theta}$$

$$\therefore \int_0^1 B(\theta | m+a, N-m+b) d\theta$$

$$= \int_0^1 \theta^{m+a-1} \cdot (1-\theta)^{N-m+b-1} \cdot \frac{\Gamma(N+a+b)}{\Gamma(m+a)\Gamma(N-m+b)} d\theta = 1$$

$$\therefore \int_0^1 \theta^{m+a-1} \cdot (1-\theta)^{N-m+b-1} d\theta = \left(\frac{\Gamma(N+a+b)}{\Gamma(m+a)\Gamma(N-m+b)} \right)^{-1}$$

Thus (*) becomes $\theta^{m+a-1} \cdot (1-\theta)^{N-m+b-1} \cdot \frac{\Gamma(N+a+b)}{\Gamma(m+a)\Gamma(N-m+b)}$

$$= B(\theta | m+a, N-m+b) \quad \#$$

2. Gamma - Poisson conjugation:

$$\text{Gamma distribution: } f(x|\alpha, \beta) = \frac{\beta^\alpha}{\Gamma(\alpha)} \cdot x^{\alpha-1} \cdot e^{-\beta x}$$

proof: By Bayes Rule, we have $P(\lambda|x) = \frac{P(x|\lambda) \cdot P(\lambda)}{P(x)}$
 $\propto P(x|\lambda) \cdot P(\lambda)$
 $\hookrightarrow x: \text{event}$

Assume there are N data points,

$$P(x|\lambda) = \prod_{i=1}^n \frac{\lambda^{x_i} e^{-\lambda}}{(x_i)!} = \frac{\lambda^{\sum x_i} \cdot e^{-n\lambda}}{\prod (x_i)!} \propto \lambda^{\sum x_i} \cdot e^{-n\lambda}$$

$$\underline{P(\lambda)} \propto \lambda^{\alpha-1} e^{-\beta\lambda} \quad (\text{prior})$$

$$\text{Thus, } P(\lambda|x) \propto \lambda^{\sum x_i} \cdot e^{-n\lambda} \cdot \lambda^{\alpha-1} \cdot e^{-\beta\lambda}$$

$$= \lambda^{n\bar{x}} \cdot \lambda^{\alpha-1} \cdot e^{-(\beta+n)\lambda}$$

$$= \lambda^{(n\bar{x} + \alpha - 1)} \cdot e^{-(\beta+n)\lambda} = \text{gamma}(n\bar{x} + \alpha, \beta + n)_{\#}$$